some valid_synth

tests/layeff/LowParseWriters.Parsers.fst
@@ -1,6 +1,8 @@
 module LowParseWriters.Parsers
 friend LowParseWriters.LowParse
 
+module B = LowStar.Buffer
+
 let get_parser_kind
   p
 = (dsnd p).kind
@@ -25,3 +27,31 @@ let make_parser_correct
 let size_correct
   p s x
 = LP.serializer_unique (get_parser p) (dsnd p).serializer s x
+
+let valid_synth_parser_eq
+  p1 p2
+= {
+  valid_synth_valid = (fun h b pos pos' -> ());
+  valid_synth_size = (fun x ->
+    LP.serializer_unique (get_parser p1) (dsnd p1).serializer (dsnd p2).serializer x
+  );
+}
+
+let parse_synth
+  p1 #t2 f2 f1
+= make_parser
+    ((dsnd p1).parser `LP.parse_synth` f2)
+    (LP.serialize_synth (dsnd p1).parser f2 (dsnd p1).serializer f1 ())
+    (LP.jump_synth (dsnd p1).jumper f2 ())
+
+let valid_synth_parse_synth
+  p1 #t2 f2 f1 sq
+= {
+  valid_synth_valid = (fun h b pos pos' ->
+    LP.valid_synth h (get_parser p1) f2 (LP.make_slice b (B.len b)) pos
+  );
+  valid_synth_size = (fun x ->
+    LP.synth_injective_synth_inverse_synth_inverse_recip f2 f1 ();
+    LP.serialize_synth_eq (get_parser p1) f2 (dsnd p1).serializer f1 () (f2 x)
+  );
+}
