tests/layeff/LowParseWriters.Parsers.fsti
@@ -1,7 +1,7 @@
 module LowParseWriters.Parsers
 include LowParseWriters
 
-module LP = LowParse.Low.Base
+module LP = LowParse.Low
 module Seq = FStar.Seq
 
 inline_for_extraction
@@ -55,3 +55,42 @@ val size_correct
   (x: dfst p)
 : Lemma
   (size p x == Seq.length (LP.serialize s x))
+
+val valid_synth_parser_eq
+  (p1: parser)
+  (p2: parser {
+    dfst p1 == dfst p2 /\
+    get_parser_kind p1 == get_parser_kind p2 /\
+    get_parser p1 == LP.coerce (LP.parser (get_parser_kind p1) (dfst p1)) (get_parser p2)
+  })
+: Tot (valid_synth_t p1 p2 (fun _ -> True) (fun x -> x))
+
+inline_for_extraction
+val parse_synth
+  (p1: parser)
+  (#t2: Type)
+  (f2: dfst p1 -> GTot t2)
+  (f1: t2 -> GTot (dfst p1))
+: Pure parser
+  (requires (
+    LP.synth_injective f2 /\
+    LP.synth_inverse f2 f1
+  ))
+  (ensures (fun r ->
+    LP.synth_injective f2 /\
+    LP.synth_inverse f2 f1 /\
+    dfst r == t2 /\
+    get_parser_kind r == get_parser_kind p1 /\
+    get_parser r == LP.coerce (LP.parser (get_parser_kind r) (dfst r)) (get_parser p1 `LP.parse_synth` f2)
+  ))
+
+val valid_synth_parse_synth
+  (p1: parser)
+  (#t2: Type)
+  (f2: dfst p1 -> GTot t2)
+  (f1: t2 -> GTot (dfst p1))
+  (sq: squash (
+    LP.synth_injective f2 /\
+    LP.synth_inverse f2 f1
+  ))
+: Tot (valid_synth_t p1 (parse_synth p1 f2 f1) (fun _ -> True) f2)
